strings: cover missing ascii whitespace chars, document limitation of Fields spec,
use `lexico` for go_string ordering, and define a simpler `split_fields`
function with no fuel.

new/golang/defn/string.v
@@ -1,128 +1,47 @@
 From New.golang.defn Require Export loop assume predeclared.
 From New.code.github_com.mit_pdos.perennial.goose.model Require Import strings.
-From Coq Require Import PropExtensionality.
 
 Module go.
 Section defs.
 Context {ext : ffi_syntax}.
 Context {go_lctx : GoLocalContext} {go_gctx : GoGlobalContext}.
 
-(* Lexicographic ordering on go_string (byte lists). *)
-Fixpoint go_string_ltb (x y : go_string) : bool :=
-  match x, y with
-  | [], [] => false
-  | [], _ => true
-  | _, [] => false
-  | (a :: x), (b :: y) => if (word.ltu a b) then
-                         true
-                       else if (word.eqb a b) then
-                              go_string_ltb x y
-                            else false
-  end.
+Global Instance w8_lexico : Lexico w8 := (λ x y, uint.Z x < uint.Z y).
+
+Global Instance : TrichotomyT (lexico (A:=w8)).
+Proof.
+  intros x y. destruct (uint.Z x ?= uint.Z y) eqn:Heq.
+  - apply Z.compare_eq in Heq. left. right. word.
+  - left. left. rewrite (Z.compare_lt_iff (uint.Z x) (uint.Z y)) in Heq.
+    rewrite /lexico /= /w8_lexico //.
+  - right. rewrite (Z.compare_gt_iff (uint.Z x) (uint.Z y)) in Heq.
+    rewrite /lexico /= /w8_lexico //.
+Defined. (* for computing bool_decide *)
+
+Global Instance : StrictOrder (lexico (A:=w8)).
+Proof.
+  constructor.
+  - intros x. rewrite /lexico /w8_lexico /complement. intros H. lia.
+  - intros x y z. rewrite /lexico /w8_lexico. lia.
+Qed.
+
+Definition go_string_lt : go_string → go_string → Prop := lexico.
+
+Instance : StrictOrder go_string_lt.
+Proof. apply _. Qed.
 
 Example go_string_ltb_examples :
-  go_string_ltb "" "" = false ∧
-  go_string_ltb "" "a" = true ∧
-  go_string_ltb "a" "" = false ∧
-  go_string_ltb "ab" "a" = false ∧
-  go_string_ltb "ab" "b" = true
-  := ltac:(auto).
-
-Fixpoint go_string_lt (x y : go_string) : Prop :=
-  match x, y with
-  | [], [] => False
-  | [], _ => True
-  | _, [] => False
-  | (a :: x), (b :: y) => if decide (uint.Z a < uint.Z b) then
-                         True
-                       else if decide (uint.Z a = uint.Z b) then
-                              go_string_lt x y
-                            else false
-  end.
+  ¬ go_string_lt "" "" ∧
+  go_string_lt "" "a" ∧
+  ¬ go_string_lt "a" "" ∧
+  ¬ go_string_lt "ab" "a" ∧
+  go_string_lt "ab" "b".
+Proof.
+  split_and!; eapply bool_decide_unpack; done.
+Qed.
 
 Definition go_string_le (x y : go_string) : Prop :=
   x = y ∨ go_string_lt x y.
-
-Definition go_string_leb (x y : go_string) : bool :=
- bool_decide(x = y) || go_string_ltb x y.
-
-(* Ordering lemmas: totality and reflexivity for w8 and go_string,
-   used to show go_string_leb is a total preorder. *)
-Lemma w8_trichotomy (a b : w8) :
-  word.ltu a b = true \/ word.eqb a b = true \/ word.ltu b a = true.
-Proof.
-  destruct (decide (uint.Z a < uint.Z b)%Z) as [Hab|Hnab].
-  - left.
-    rewrite word.unsigned_ltu.
-    apply Z.ltb_lt.
-    exact Hab.
-  - destruct (decide (uint.Z a = uint.Z b)%Z) as [Heq|Hneq].
-    + right. left.
-      apply word.eqb_eq. 
-      word.
-    + right. right.
-      assert ((uint.Z b < uint.Z a)%Z) by lia.
-      rewrite word.unsigned_ltu.
-      apply Z.ltb_lt.
-      assumption.
-Qed.
-
-Lemma w8_ltu_irrefl (a : w8) :
-  word.ltu a a = false.
-Proof.
-  rewrite word.unsigned_ltu. 
-  apply Z.ltb_irrefl.
-Qed.
-
-Lemma w8_eqb_refl (a : w8) :
-  word.eqb a a = true.
-Proof.
-  apply word.eqb_eq. done.
-Qed.
-
-Lemma go_string_ltb_total x y :
-  x = y \/ go_string_ltb x y = true \/ go_string_ltb y x = true.
-Proof.
-  revert y.
-  induction x as [|a x IH]; intros [|b y].
-  - left; reflexivity.
-  - right; left; reflexivity.
-  - right; right; reflexivity.
-  - destruct (w8_trichotomy a b) as [Hlt | [Heq | Hgt]].
-    + right; left; simpl; rewrite Hlt; reflexivity.
-    + destruct (word.eqb_spec a b) as [Hab | Hab].
-      * subst.
-        destruct (IH y) as [Hxy | [Hxy | Hxy]].
-        -- left; congruence.
-        -- right; left; simpl; rewrite w8_ltu_irrefl. rewrite w8_eqb_refl; assumption.
-        -- right; right; simpl; rewrite w8_ltu_irrefl. rewrite w8_eqb_refl; assumption.
-      * exfalso. apply Hab. done.
-    + right; right; simpl; rewrite Hgt; reflexivity.
-Qed.
-
-Lemma go_string_leb_total x y :
-  go_string_leb x y = true \/ go_string_leb y x = true.
-Proof.
-  destruct (go_string_ltb_total x y) as [-> | [Hxy | Hyx]].
-  - left.
-    unfold go_string_leb.
-    assert (y = y) by done. 
-    assert (bool_decide (y = y)) by set_solver.  
-    replace (bool_decide (y = y)) with true.
-    { done. } rewrite bool_decide_true. { done. } done.
-  - left.
-    unfold go_string_leb.
-    replace (go_string_ltb x y ) with true. 
-    replace (true = true) with True;first lia. 
-    apply Coq.Logic.PropExtensionality.propositional_extensionality; naive_solver.
-  
-  - right.
-    unfold go_string_leb.
-
-    rewrite Hyx. 
-    replace (true = true) with True;first lia. 
-    apply Coq.Logic.PropExtensionality.propositional_extensionality; naive_solver.
-Qed.
 
 Class StringSemantics `{!GoSemanticsFunctions} :=
 {
@@ -152,16 +71,16 @@ Class StringSemantics `{!GoSemanticsFunctions} :=
     ⟦Convert from to, v⟧ ⤳[internal] (@! strings.StringToByteSlice v);
 
   #[global] lt_string (x y : go_string) ::
-    ⟦GoOp GoLt go.string, (#x, #y)⟧ ⤳[under] #(go_string_ltb x y);
+    ⟦GoOp GoLt go.string, (#x, #y)⟧ ⤳[under] #(bool_decide (go_string_lt x y));
 
   #[global] le_string (x y : go_string) ::
-    ⟦GoOp GoLe go.string, (#x, #y)⟧ ⤳[under] #(go_string_leb x y);
+    ⟦GoOp GoLe go.string, (#x, #y)⟧ ⤳[under] #(bool_decide (go_string_le x y));
 
   #[global] gt_string (x y : go_string) ::
-    ⟦GoOp GoGt go.string, (#x, #y)⟧ ⤳[under] #(go_string_ltb y x);
+    ⟦GoOp GoGt go.string, (#x, #y)⟧ ⤳[under] #(bool_decide (go_string_lt y x));
 
   #[global] ge_string (x y : go_string) ::
-    ⟦GoOp GoGe go.string, (#x, #y)⟧ ⤳[under] #(go_string_leb y x);
+    ⟦GoOp GoGe go.string, (#x, #y)⟧ ⤳[under] #(bool_decide (go_string_le y x));
 }.
 End defs.
 End go.
