new/proof/strings.v
@@ -1,5 +1,4 @@
 From New.proof Require Import proof_prelude.
-From New.proof Require Export std.
 From New.generatedproof Require Export strings.
 From Perennial Require Import base.
 
@@ -19,7 +18,6 @@ Lemma wp_asciiSpace_init :
 Proof.
 Admitted.
 
-
 Lemma wp_initialize' get_is_pkg_init :
   get_is_pkg_init_prop strings get_is_pkg_init →
   {{{ own_initializing get_is_pkg_init }}}
@@ -34,71 +32,54 @@ Proof.
   iEval (rewrite is_pkg_init_unfold /=). iFrame "∗#". done.
 Qed.
 
-(* Pure model of strings.Fields:
-   is_space_byte identifies ASCII whitespace bytes (space, \t, \n, \r);
-   drop_while/take_while are helpers used to define split_fields_go,
-   which models Go's strings.Fields splitting behavior.
-   fields_spec ties the axiomatic WP to the pure model. *)
-Definition is_space_byte (b : w8) : bool :=
-  (word.eqb b (W8 32)) ||    (* space    *)
-  (word.eqb b (W8 9))  ||    (* \t       *)
-  (word.eqb b (W8 10)) ||    (* \n       *)
-  (word.eqb b (W8 13)).      (* \r       *)
+(* Model for Go's unicode.IsSpace for ASCII-range bytes.
+   Based on https://cs.opensource.google/go/go/+/refs/tags/go1.26.1:src/strings/strings.go;l=377 *)
+Definition is_ascii_space (b : w8) : bool :=
+  (word.eqb b (W8 9))  ||    (* \t  (0x09) *)
+  (word.eqb b (W8 10)) ||    (* \n  (0x0A) *)
+  (word.eqb b (W8 11)) ||    (* \v  (0x0B) *)
+  (word.eqb b (W8 12)) ||    (* \f  (0x0C) *)
+  (word.eqb b (W8 13)) ||    (* \r  (0x0D) *)
+  (word.eqb b (W8 32))      (* space (0x20) *)
+.
 
-Fixpoint drop_while {A} (f : A -> bool) (xs : list A) : list A :=
-  match xs with
-  | [] => []
-  | x :: xs' => if f x then drop_while f xs' else x :: xs'
+Fixpoint split_fields_aux (s : go_string) (w : option go_string) : list go_string :=
+  match s with
+  | [] => match w with None => [] | Some w => [w] end
+  | x :: s => if is_ascii_space x then
+              match w with
+              | None => split_fields_aux s None
+              | Some w => w :: split_fields_aux s None
+              end
+            else split_fields_aux s (Some (default [] w ++ [x]))
   end.
+Definition split_fields (s : go_string) : list go_string := split_fields_aux s None.
 
-Fixpoint take_while {A} (f : A -> bool) (xs : list A) : list A :=
-  match xs with
-  | [] => []
-  | x :: xs' => if f x then x :: take_while f xs' else []
-  end.
-
-Fixpoint split_fields_go (fuel : nat) (s : go_string) : list go_string :=
-  match fuel with
-  | O => []
-  | S fuel' =>
-      let s' := drop_while is_space_byte s in
-      match s' with
-      | [] => []
-      | _ =>
-          let w := take_while (fun b => negb (is_space_byte b)) s' in
-          let rest := drop_while (fun b => negb (is_space_byte b)) s' in
-          w :: split_fields_go fuel' rest
-      end
-  end.
-
-Definition fields_spec (s : go_string) (ss : list go_string) : Prop :=
-  ss = split_fields_go (length s) s ∧ (length ss) < 2 ^ 64 .
-
-Axiom wp_strings_Fields :
+(* FIXME: this is wrong (unsound) for strings with non-ascii runes. Simplest
+   solution might be to add a precondition for the string to be all ascii. *)
+Axiom wp_Fields :
   ∀ `{!strings.Assumptions} (s : go_string),
   {{{ is_pkg_init strings }}}
     @! strings.Fields #s
-  {{{ sl (ss : list go_string),
+  {{{ sl,
       RET #sl;
-      sl ↦* ss ∗ ⌜ fields_spec s ss ⌝ ∗  own_slice_cap w8 sl (DfracOwn 1) }}}.
+      sl ↦* (split_fields s) ∗ own_slice_cap w8 sl (DfracOwn 1) }}}.
 
-(* Unit tests for split_fields_go *)
-Example split_fields_go_hello :
-  split_fields_go (length "hello"%go) "hello"%go = ["hello"%go].
+(* Test split_fields because it is part of the wp_Fields axiom. *)
+Example split_fields_hello :
+  split_fields "hello"%go = ["hello"%go].
 Proof. vm_compute. reflexivity. Qed.
 
-Example split_fields_go_leading_spaces :
-  split_fields_go (length "   hello world"%go) "   hello world"%go =
-    ["hello"%go; "world"%go].
+Example split_fields_leading_spaces :
+  split_fields "   hello world"%go = ["hello"%go; "world"%go].
 Proof. vm_compute. reflexivity. Qed.
 
-Example split_fields_go_two_words :
-  split_fields_go (length "hello world"%go) "hello world"%go =
-    ["hello"%go; "world"%go].
+Example split_fields_two_words :
+  split_fields "hello world"%go = ["hello"%go; "world"%go].
 Proof. vm_compute. reflexivity. Qed.
 
-Example split_fields_go_empty :
-  split_fields_go (length ""%go) ""%go = [].
+Example split_fields_empty :
+  split_fields ""%go = [].
 Proof. vm_compute. reflexivity. Qed.
 
 Definition bs_tab : w8 := W8 9.
@@ -109,18 +90,17 @@ Definition bs_sp  : w8 := W8 32.
 Definition hello_world_ws : go_string :=
   [bs_sp; bs_tab] ++ "hello"%go ++ [bs_nl] ++ "world"%go ++ [bs_cr; bs_sp].
 
-Example split_fields_go_mixed_ws :
-  split_fields_go (length hello_world_ws) hello_world_ws =
+Example split_fields_mixed_ws :
+  split_fields hello_world_ws =
     ["hello"%go; "world"%go].
 Proof. vm_compute. reflexivity. Qed.
 
-Example split_fields_go_interp_string_literal :
-  split_fields_go (length "  hello\tthere\ngeneral\rkenobi "%go)
-                  "  hello\tthere\ngeneral\rkenobi "%go
+Example split_fields_interp_string_literal :
+  split_fields "  hello\tthere\ngeneral\rkenobi "%go
   = ["hello"%go; "there"%go; "general"%go; "kenobi"%go].
 Proof. vm_compute. reflexivity. Qed.
 
-(* Unit tests for wp_strings_Fields, exercising the axiom via fields_spec *)
+(* Unit tests for wp_Fields, exercising the axiom via fields_spec *)
 Example wp_Fields_mixed_ws :
   {{{ is_pkg_init strings }}}
     @! strings.Fields #("  hello\tthere\ngeneral\rkenobi "%go)
@@ -129,10 +109,8 @@ Example wp_Fields_mixed_ws :
       sl ↦* ["hello"%go; "there"%go; "general"%go; "kenobi"%go] ∗ own_slice_cap w8 sl (DfracOwn 1) }}}.
 Proof.
   iIntros (Φ) "#Hinit HΦ".
-  wp_apply (wp_strings_Fields).
-  iIntros (sl ss) "(Hsl & %Hspec & Hcap)".
-  destruct Hspec as [Hss _].
-  subst ss.
+  wp_apply (wp_Fields).
+  iIntros (sl) "(Hsl & Hcap)".
   iApply "HΦ". iFrame.
 Qed.
 
@@ -142,14 +120,12 @@ Example wp_Fields_two_words:
   {{{ sl,
       RET #sl;
       sl ↦* ["hello"%go; "world"%go] ∗
-      own_slice_cap w8 sl (DfracOwn 1) 
+      own_slice_cap w8 sl (DfracOwn 1)
   }}}.
 Proof.
   iIntros (Φ) "#Hinit HΦ".
-  wp_apply (wp_strings_Fields "hello world"%go).
-  iIntros (sl ss) "(Hsl & %Hspec & Hcap)".
-  destruct Hspec as [Hss _].
-  subst ss.
+  wp_apply (wp_Fields "hello world"%go).
+  iIntros (sl) "(Hsl & Hcap)".
   iApply "HΦ". iFrame.
 Qed.
 
